wip

code/bignum/Hacl.Bignum.ExpFW.fst
@@ -1,4 +1,4 @@
-module Hacl.Bignum.ExponentiationPrecomp
+module Hacl.Bignum.ExpFW
 
 open FStar.HyperStack
 open FStar.HyperStack.ST
@@ -13,16 +13,16 @@ module ST = FStar.HyperStack.ST
 module LSeq = Lib.Sequence
 module Loops = Lib.LoopCombinators
 
-module S = Hacl.Spec.Bignum.ExponentiationPrecomp
+module S = Hacl.Spec.Bignum.ExpFW
 module SN = Hacl.Spec.Bignum
 module SM = Hacl.Spec.Bignum.Montgomery
 module BB = Hacl.Spec.Bignum.Base
 
 module BN = Hacl.Bignum
 module BM = Hacl.Bignum.Montgomery
+module EBM = Hacl.Bignum.ExpBM
 
-friend Hacl.Spec.Bignum.ExponentiationPrecomp
-friend Hacl.Bignum.Exponentiation
+friend Hacl.Spec.Bignum.ExpFW
 
 #reset-options "--z3rlimit 150 --fuel 0 --ifuel 0"
 
@@ -431,86 +431,3 @@ let bn_mod_exp_fw_precompr2 #t k n a bBits b l r2 res =
 let bn_mod_exp_fw_precompr2_ct #t k n a bBits b l r2 res =
   bn_mod_exp_fw_precompr2_ #t k
     (bn_mod_exp_fw_mont_f k) (bn_mod_exp_fw_mont_rem k) n a bBits b l r2 res
-
-
-let bn_mod_exp_fw #t k bn_mod_exp_fw_precompr2 nBits n a bBits b l res =
-  [@inline_let] let len = k.BM.bn.BN.len in
-  push_frame ();
-  let r2 = create len (uint #t #SEC 0) in
-  BM.precomp nBits n r2;
-  bn_mod_exp_fw_precompr2 n a bBits b l r2 res;
-  pop_frame ()
-
-
-let bn_mod_exp_fw_ct #t k bn_mod_exp_fw_precompr2_ct nBits n a bBits b l res =
-  [@inline_let] let len = k.BM.bn.BN.len in
-  push_frame ();
-  let r2 = create len (uint #t #SEC 0) in
-  BM.precomp nBits n r2;
-  bn_mod_exp_fw_precompr2_ct n a bBits b l r2 res;
-  pop_frame ()
-
-
-[@CInline]
-let bn_mod_exp_fw_precompr2_u32 (len:BN.meta_len U32) : bn_mod_exp_fw_precompr2_st U32 len =
-  bn_mod_exp_fw_precompr2 (BM.mk_runtime_mont len)
-[@CInline]
-let bn_mod_exp_fw_precompr2_ct_u32 (len:BN.meta_len U32) : bn_mod_exp_fw_precompr2_st U32 len =
-  bn_mod_exp_fw_precompr2_ct (BM.mk_runtime_mont len)
-[@CInline]
-let bn_mod_exp_fw_u32 (len:BN.meta_len U32) : bn_mod_exp_fw_st U32 len =
-  bn_mod_exp_fw (BM.mk_runtime_mont len) (bn_mod_exp_fw_precompr2_u32 len)
-[@CInline]
-let bn_mod_exp_fw_ct_u32 (len:BN.meta_len U32) : bn_mod_exp_fw_st U32 len =
-  bn_mod_exp_fw_ct (BM.mk_runtime_mont len) (bn_mod_exp_fw_precompr2_ct_u32 len)
-
-inline_for_extraction noextract
-let mk_runtime_exp_u32 (len: BN.meta_len U32) : exp U32 = {
-  mont = BM.mk_runtime_mont len;
-  exp_check = BE.bn_check_mod_exp_u32 len;
-  mod_exp_precomp = BE.bn_mod_exp_precompr2_u32 len;
-  ct_mod_exp_precomp = BE.bn_mod_exp_mont_ladder_precompr2_u32 len;
-  mod_exp = BE.bn_mod_exp_u32 len;
-  ct_mod_exp = BE.bn_mod_exp_mont_ladder_u32 len;
-  mod_exp_fw_precomp = bn_mod_exp_fw_precompr2_u32 len;
-  ct_mod_exp_fw_precomp = bn_mod_exp_fw_precompr2_ct_u32 len;
-  mod_exp_fw = bn_mod_exp_fw_u32 len;
-  ct_mod_exp_fw = bn_mod_exp_fw_ct_u32 len;
-  }
-
-
-[@CInline]
-let bn_mod_exp_fw_precompr2_u64 (len:BN.meta_len U64) : bn_mod_exp_fw_precompr2_st U64 len =
-  bn_mod_exp_fw_precompr2 (BM.mk_runtime_mont len)
-[@CInline]
-let bn_mod_exp_fw_precompr2_ct_u64 (len:BN.meta_len U64) : bn_mod_exp_fw_precompr2_st U64 len =
-  bn_mod_exp_fw_precompr2_ct (BM.mk_runtime_mont len)
-[@CInline]
-let bn_mod_exp_fw_u64 (len:BN.meta_len U64) : bn_mod_exp_fw_st U64 len =
-  bn_mod_exp_fw (BM.mk_runtime_mont len) (bn_mod_exp_fw_precompr2_u64 len)
-[@CInline]
-let bn_mod_exp_fw_ct_u64 (len:BN.meta_len U64) : bn_mod_exp_fw_st U64 len =
-  bn_mod_exp_fw_ct (BM.mk_runtime_mont len) (bn_mod_exp_fw_precompr2_ct_u64 len)
-
-inline_for_extraction noextract
-let mk_runtime_exp_u64 (len: BN.meta_len U64) : exp U64 = {
-  mont = BM.mk_runtime_mont len;
-  exp_check = BE.bn_check_mod_exp_u64 len;
-  mod_exp_precomp = BE.bn_mod_exp_precompr2_u64 len;
-  ct_mod_exp_precomp = BE.bn_mod_exp_mont_ladder_precompr2_u64 len;
-  mod_exp = BE.bn_mod_exp_u64 len;
-  ct_mod_exp = BE.bn_mod_exp_mont_ladder_u64 len;
-  mod_exp_fw_precomp = bn_mod_exp_fw_precompr2_u64 len;
-  ct_mod_exp_fw_precomp = bn_mod_exp_fw_precompr2_ct_u64 len;
-  mod_exp_fw = bn_mod_exp_fw_u64 len;
-  ct_mod_exp_fw = bn_mod_exp_fw_ct_u64 len;
-  }
-
-
-let mk_runtime_exp (#t:limb_t) (len:BN.meta_len t) : exp t =
-  match t with
-  | U32 -> mk_runtime_exp_u32 len
-  | U64 -> mk_runtime_exp_u64 len
-
-let mk_runtime_exp_len_lemma #t len =
-  BM.mk_runtime_mont_len_lemma #t len
