code/bignum/Hacl.Bignum.Exponentiation.fst
@@ -17,213 +17,12 @@ module S = Hacl.Spec.Bignum.Exponentiation
 module LSeq = Lib.Sequence
 module Loops = Lib.LoopCombinators
 
+include Hacl.Bignum.ExpBM
+include Hacl.Bignum.ExpFW
+
 friend Hacl.Spec.Bignum.Exponentiation
 
-
 #reset-options "--z3rlimit 50 --fuel 0 --ifuel 0"
-
-let bn_check_mod_exp #t k n a bBits b =
-  [@inline_let] let len = k.BM.bn.BN.len in
-  let m0 = k.BM.mont_check n in
-  let bLen = blocks bBits (size (bits t)) in
-  let m1 = BN.bn_is_zero_mask bLen b in
-  let m1' = lognot m1 in
-  let m2 =
-    if bBits <. size (bits t) *! bLen
-    then BN.bn_lt_pow2_mask bLen b bBits
-    else ones t SEC in
-  let m3 = BN.bn_lt_mask len a n in
-  let m = m1' &. m2 &. m3 in
-  m0 &. m
-
-
-inline_for_extraction noextract
-let bn_mod_exp_loop_st (t:limb_t) (nLen:BN.meta_len t) =
-    n:lbignum t nLen
-  -> nInv:limb t
-  -> bBits:size_t{v bBits > 0}
-  -> bLen:size_t{v bLen = v (blocks bBits (size (bits t))) /\ (v bBits - 1) / bits t < v bLen}
-  -> b:lbignum t bLen
-  -> aM:lbignum t nLen
-  -> accM:lbignum t nLen ->
-  Stack unit
-  (requires fun h ->
-    live h n /\ live h b /\ live h aM /\ live h accM /\
-    disjoint aM accM /\ disjoint aM b /\ disjoint aM n /\
-    disjoint accM b /\ disjoint accM n)
-  (ensures  fun h0 _ h1 -> modifies (loc aM |+| loc accM) h0 h1 /\
-    (as_seq h1 aM, as_seq h1 accM) ==
-      Loops.repeati (v bBits)
-	(S.bn_mod_exp_f (as_seq h0 n) nInv (v bBits) (v bLen) (as_seq h0 b))
-      (as_seq h0 aM, as_seq h0 accM))
-
-
-inline_for_extraction noextract
-val bn_mod_exp_loop: #t:limb_t -> k:BM.mont t -> bn_mod_exp_loop_st t k.BM.bn.BN.len
-let bn_mod_exp_loop #t k n nInv bBits bLen b aM accM =
-  [@inline_let]
-  let spec h0 = S.bn_mod_exp_f (as_seq h0 n) nInv (v bBits) (v bLen) (as_seq h0 b) in
-  let h0 = ST.get () in
-  loop2 h0 bBits aM accM spec
-  (fun i ->
-    Loops.unfold_repeati (v bBits) (spec h0) (as_seq h0 aM, as_seq h0 accM) (v i);
-    let get_bit = BN.bn_get_ith_bit bLen b i in
-
-    if not (Hacl.Bignum.Base.unsafe_bool_of_limb0 get_bit) then
-      BM.mul n nInv aM accM accM; // acc = (acc * a) % n
-    BM.sqr n nInv aM aM // a = (a * a) % n
-  )
-
-
-inline_for_extraction noextract
-let bn_mod_exp_mont_st (t:limb_t) (len:BN.meta_len t) =
-    n:lbignum t len
-  -> a:lbignum t len
-  -> acc:lbignum t len
-  -> bBits:size_t{v bBits > 0}
-  -> b:lbignum t (blocks bBits (size (bits t)))
-  -> r2:lbignum t len
-  -> res:lbignum t len ->
-  Stack unit
-  (requires fun h ->
-    live h n /\ live h a /\ live h b /\ live h res /\ live h acc /\ live h r2 /\
-    disjoint res a /\ disjoint res b /\ disjoint res n /\ disjoint res acc /\
-    disjoint a n /\ disjoint acc n /\ disjoint res r2 /\ disjoint r2 a /\
-    disjoint r2 acc /\ disjoint r2 n)
-  (ensures  fun h0 _ h1 -> modifies (loc res) h0 h1 /\
-    as_seq h1 res ==
-    S.bn_mod_exp_mont (v len) (as_seq h0 n) (as_seq h0 a) (as_seq h0 acc) (v bBits) (as_seq h0 b) (as_seq h0 r2))
-
-
-inline_for_extraction noextract
-val bn_mod_exp_mont: #t:limb_t -> k:BM.mont t -> bn_mod_exp_mont_st t k.BM.bn.BN.len
-let bn_mod_exp_mont #t k n a acc bBits b r2 res =
-  [@inline_let] let len = k.BM.bn.BN.len in
-  push_frame ();
-  let bLen = blocks bBits (size (bits t)) in
-  let nInv = BM.mod_inv_limb n.(0ul) in // n * nInv = 1 (mod (pow2 64))
-
-  let aM   = create len (uint #t #SEC 0) in
-  let accM = create len (uint #t #SEC 0) in
-  BM.to n nInv r2 a aM;
-  BM.to n nInv r2 acc accM;
-  bn_mod_exp_loop k n nInv bBits bLen b aM accM;
-  BM.from n nInv accM res;
-  pop_frame ()
-
-
-let bn_mod_exp_precompr2 #t k n a bBits b r2 res =
-  [@inline_let] let len = k.BM.bn.BN.len in
-  push_frame ();
-  let acc  = create len (uint #t #SEC 0) in
-  BN.bn_from_uint len (uint #t #SEC 1) acc;
-  bn_mod_exp_mont k n a acc bBits b r2 res;
-  pop_frame ()
-
-///
-///  Montgomery ladder for exponentiation
-///
-
-inline_for_extraction noextract
-let bn_mod_exp_mont_ladder_loop_st (t:limb_t) (len:BN.meta_len t) =
-    n:lbignum t len
-  -> nInv:limb t
-  -> bBits:size_t{v bBits > 0}
-  -> bLen:size_t{v bLen = v (blocks bBits (size (bits t))) /\ (v bBits - 1) / bits t < v bLen}
-  -> b:lbignum t bLen
-  -> rM0:lbignum t len
-  -> rM1:lbignum t len
-  -> sw:lbignum t 1ul ->
-  Stack unit
-  (requires fun h ->
-    live h n /\ live h b /\ live h rM0 /\ live h rM1 /\ live h sw /\
-    disjoint rM0 rM1 /\ disjoint rM0 b /\ disjoint rM0 n /\
-    disjoint rM1 b /\ disjoint rM1 n /\
-    disjoint sw rM0 /\ disjoint sw rM1 /\ disjoint sw b /\ disjoint sw n)
-  (ensures  fun h0 _ h1 -> modifies (loc rM0 |+| loc rM1 |+| loc sw) h0 h1 /\
-    (as_seq h1 rM0, as_seq h1 rM1, LSeq.index (as_seq h1 sw) 0) ==
-      Loops.repeat_gen (v bBits) (S.bn_mod_exp_mont_ladder_t t (v len) (v bBits))
-	(S.bn_mod_exp_mont_ladder_f (as_seq h0 n) nInv (v bBits) (v bLen) (as_seq h0 b))
-      (as_seq h0 rM0, as_seq h0 rM1, LSeq.index (as_seq h0 sw) 0))
-
-
-inline_for_extraction noextract
-val bn_mod_exp_mont_ladder_loop: #t:limb_t -> k:BM.mont t -> bn_mod_exp_mont_ladder_loop_st t k.BM.bn.BN.len
-let bn_mod_exp_mont_ladder_loop #t k n nInv bBits bLen b rM0 rM1 sw =
-  [@inline_let] let len = k.BM.bn.BN.len in
-  [@inline_let]
-  let refl h i : GTot (S.bn_mod_exp_mont_ladder_t t (v len) (v bBits) i) =
-    (as_seq h rM0, as_seq h rM1, LSeq.index (as_seq h sw) 0) in
-  [@inline_let]
-  let footprint i = loc rM0 |+| loc rM1 |+| loc sw in
-  [@inline_let]
-  let spec h0 = S.bn_mod_exp_mont_ladder_f (as_seq h0 n) nInv (v bBits) (v bLen) (as_seq h0 b) in
-  let h0 = ST.get () in
-  loop h0 bBits (S.bn_mod_exp_mont_ladder_t t (v len) (v bBits)) refl footprint spec
-  (fun i ->
-    Loops.unfold_repeat_gen (v bBits)
-      (S.bn_mod_exp_mont_ladder_t t (v len) (v bBits)) (spec h0) (refl h0 0) (v i);
-    let bit = BN.bn_get_ith_bit bLen b (bBits -! i -! 1ul) in
-    let sw1 = bit ^. sw.(0ul) in
-    BN.cswap2 len sw1 rM0 rM1;
-    BM.mul n nInv rM1 rM0 rM1;
-    BM.sqr n nInv rM0 rM0;
-    sw.(0ul) <- bit
-  );
-  let h1 = ST.get () in
-  assert (refl h1 (v bBits) == Loops.repeat_gen (v bBits)
-    (S.bn_mod_exp_mont_ladder_t t (v len) (v bBits)) (spec h0) (refl h0 0))
-
-
-inline_for_extraction noextract
-let bn_mod_exp_mont_ladder_st1 (t:limb_t) (len:BN.meta_len t) =
-    n:lbignum t len
-  -> a:lbignum t len
-  -> acc:lbignum t len
-  -> bBits:size_t{v bBits > 0}
-  -> b:lbignum t (blocks bBits (size (bits t)))
-  -> r2:lbignum t len
-  -> res:lbignum t len ->
-  Stack unit
-  (requires fun h ->
-    live h n /\ live h a /\ live h b /\ live h res /\ live h acc /\ live h r2 /\
-    disjoint res a /\ disjoint res b /\ disjoint res n /\ disjoint res acc /\
-    disjoint a n /\ disjoint acc n /\ disjoint r2 a /\ disjoint r2 res /\
-    disjoint r2 acc /\ disjoint r2 n)
-  (ensures  fun h0 _ h1 -> modifies (loc res) h0 h1 /\
-    as_seq h1 res ==
-      S.bn_mod_exp_mont_ladder_ (v len) (as_seq h0 n) (as_seq h0 a)
-	(as_seq h0 acc) (v bBits) (as_seq h0 b) (as_seq h0 r2))
-
-
-inline_for_extraction noextract
-val bn_mod_exp_mont_ladder_: #t:limb_t -> k:BM.mont t -> bn_mod_exp_mont_ladder_st1 t k.BM.bn.BN.len
-let bn_mod_exp_mont_ladder_ #t k n a one bBits b r2 res =
-  [@inline_let] let len = k.BM.bn.BN.len in
-  push_frame ();
-  let bLen = blocks bBits (size (bits t)) in
-  let nInv = BM.mod_inv_limb n.(0ul) in // n * nInv = 1 (mod (pow2 64))
-
-  let rM0 = create len (uint #t #SEC 0) in
-  let rM1 = create len (uint #t #SEC 0) in
-  let sw  = create 1ul (uint #t #SEC 0) in
-  BM.to n nInv r2 one rM0;
-  BM.to n nInv r2 a rM1;
-
-  bn_mod_exp_mont_ladder_loop k n nInv bBits bLen b rM0 rM1 sw;
-  BN.cswap2 len sw.(0ul) rM0 rM1;
-  BM.from n nInv rM0 res;
-  pop_frame ()
-
-
-let bn_mod_exp_mont_ladder_precompr2 #t k n a bBits b r2 res =
-  [@inline_let] let len = k.BM.bn.BN.len in
-  push_frame ();
-  let one  = create len (uint #t 0) in
-  BN.bn_from_uint len (uint #t 1) one;
-  bn_mod_exp_mont_ladder_ k n a one bBits b r2 res;
-  pop_frame ()
-
 
 let bn_mod_exp #t k bn_mod_exp_precompr2 nBits n a bBits b res =
   [@inline_let] let len = k.BM.bn.BN.len in
@@ -243,6 +42,24 @@ let bn_mod_exp_mont_ladder #t k bn_mod_exp_mont_ladder_precompr2 nBits n a bBits
   pop_frame ()
 
 
+let bn_mod_exp_fw #t k bn_mod_exp_fw_precompr2 nBits n a bBits b l res =
+  [@inline_let] let len = k.BM.bn.BN.len in
+  push_frame ();
+  let r2 = create len (uint #t #SEC 0) in
+  BM.precomp nBits n r2;
+  bn_mod_exp_fw_precompr2 n a bBits b l r2 res;
+  pop_frame ()
+
+
+let bn_mod_exp_fw_ct #t k bn_mod_exp_fw_precompr2_ct nBits n a bBits b l res =
+  [@inline_let] let len = k.BM.bn.BN.len in
+  push_frame ();
+  let r2 = create len (uint #t #SEC 0) in
+  BM.precomp nBits n r2;
+  bn_mod_exp_fw_precompr2_ct n a bBits b l r2 res;
+  pop_frame ()
+
+
 /// A fully runtime implementation of modular exponentiation.
 
 [@CInline]
@@ -252,14 +69,24 @@ let bn_check_mod_exp_u32 (len:BN.meta_len U32) : bn_check_mod_exp_st U32 len =
 let bn_mod_exp_precompr2_u32 (len:BN.meta_len U32) : bn_mod_exp_precompr2_st U32 len =
   bn_mod_exp_precompr2 (BM.mk_runtime_mont len)
 [@CInline]
-let bn_mod_exp_mont_ladder_precompr2_u32 (len: BN.meta_len U32) : bn_mod_exp_mont_ladder_precompr2_st U32 len =
+let bn_mod_exp_mont_ladder_precompr2_u32 (len:BN.meta_len U32) : bn_mod_exp_mont_ladder_precompr2_st U32 len =
   bn_mod_exp_mont_ladder_precompr2 (BM.mk_runtime_mont len)
 [@CInline]
-let bn_mod_exp_u32 (len:BN.meta_len U32) : bn_mod_exp_st U32 len =
-  bn_mod_exp (BM.mk_runtime_mont len) (bn_mod_exp_precompr2_u32 len)
+let bn_mod_exp_fw_precompr2_u32 (len:BN.meta_len U32) : bn_mod_exp_fw_precompr2_st U32 len =
+  bn_mod_exp_fw_precompr2 (BM.mk_runtime_mont len)
 [@CInline]
-let bn_mod_exp_mont_ladder_u32 (len:BN.meta_len U32) : bn_mod_exp_mont_ladder_st U32 len =
-  bn_mod_exp_mont_ladder (BM.mk_runtime_mont len) (bn_mod_exp_mont_ladder_precompr2_u32 len)
+let bn_mod_exp_fw_precompr2_ct_u32 (len:BN.meta_len U32) : bn_mod_exp_fw_precompr2_st U32 len =
+  bn_mod_exp_fw_precompr2_ct (BM.mk_runtime_mont len)
+
+inline_for_extraction noextract
+let mk_runtime_exp_u32 (len:BN.meta_len U32) : exp U32 = {
+  mont = BM.mk_runtime_mont len;
+  exp_check = bn_check_mod_exp_u32 len;
+  mod_exp_precomp = bn_mod_exp_precompr2_u32 len;
+  ct_mod_exp_precomp = bn_mod_exp_mont_ladder_precompr2_u32 len;
+  mod_exp_fw_precomp = bn_mod_exp_fw_precompr2_u32 len;
+  ct_mod_exp_fw_precomp = bn_mod_exp_fw_precompr2_ct_u32 len;
+  }
 
 
 [@CInline]
@@ -269,11 +96,30 @@ let bn_check_mod_exp_u64 (len:BN.meta_len U64) : bn_check_mod_exp_st U64 len =
 let bn_mod_exp_precompr2_u64 (len:BN.meta_len U64) : bn_mod_exp_precompr2_st U64 len =
   bn_mod_exp_precompr2 (BM.mk_runtime_mont len)
 [@CInline]
-let bn_mod_exp_mont_ladder_precompr2_u64 (len: BN.meta_len U64) : bn_mod_exp_mont_ladder_precompr2_st U64 len =
+let bn_mod_exp_mont_ladder_precompr2_u64 (len:BN.meta_len U64) : bn_mod_exp_mont_ladder_precompr2_st U64 len =
   bn_mod_exp_mont_ladder_precompr2 (BM.mk_runtime_mont len)
 [@CInline]
-let bn_mod_exp_u64 (len:BN.meta_len U64) : bn_mod_exp_st U64 len =
-  bn_mod_exp (BM.mk_runtime_mont len) (bn_mod_exp_precompr2_u64 len)
+let bn_mod_exp_fw_precompr2_u64 (len:BN.meta_len U64) : bn_mod_exp_fw_precompr2_st U64 len =
+  bn_mod_exp_fw_precompr2 (BM.mk_runtime_mont len)
 [@CInline]
-let bn_mod_exp_mont_ladder_u64 (len:BN.meta_len U64) : bn_mod_exp_mont_ladder_st U64 len =
-  bn_mod_exp_mont_ladder (BM.mk_runtime_mont len) (bn_mod_exp_mont_ladder_precompr2_u64 len)
+let bn_mod_exp_fw_precompr2_ct_u64 (len:BN.meta_len U64) : bn_mod_exp_fw_precompr2_st U64 len =
+  bn_mod_exp_fw_precompr2_ct (BM.mk_runtime_mont len)
+
+inline_for_extraction noextract
+let mk_runtime_exp_u64 (len:BN.meta_len U64) : exp U64 = {
+  mont = BM.mk_runtime_mont len;
+  exp_check = bn_check_mod_exp_u64 len;
+  mod_exp_precomp = bn_mod_exp_precompr2_u64 len;
+  ct_mod_exp_precomp = bn_mod_exp_mont_ladder_precompr2_u64 len;
+  mod_exp_fw_precomp = bn_mod_exp_fw_precompr2_u64 len;
+  ct_mod_exp_fw_precomp = bn_mod_exp_fw_precompr2_ct_u64 len;
+  }
+
+
+let mk_runtime_exp (#t:limb_t) (len:BN.meta_len t) : exp t =
+  match t with
+  | U32 -> mk_runtime_exp_u32 len
+  | U64 -> mk_runtime_exp_u64 len
+
+let mk_runtime_exp_len_lemma #t len =
+  BM.mk_runtime_mont_len_lemma #t len
