code/bignum/Hacl.Bignum.Exponentiation.fsti
@@ -13,71 +13,10 @@ module S = Hacl.Spec.Bignum.Exponentiation
 module BN = Hacl.Bignum
 module BM = Hacl.Bignum.Montgomery
 
+include Hacl.Bignum.ExpBM
+include Hacl.Bignum.ExpFW
+
 #reset-options "--z3rlimit 50 --fuel 0 --ifuel 0"
-
-
-inline_for_extraction noextract
-let bn_check_mod_exp_st (t:limb_t) (len:BN.meta_len t) =
-    n:lbignum t len
-  -> a:lbignum t len
-  -> bBits:size_t{0 < v bBits /\ bits t * v (blocks bBits (size (bits t))) <= max_size_t}
-  -> b:lbignum t (blocks bBits (size (bits t))) ->
-  Stack (limb t)
-  (requires fun h ->
-    live h n /\ live h a /\ live h b)
-  (ensures  fun h0 r h1 -> modifies0 h0 h1 /\
-    r == S.bn_check_mod_exp (as_seq h0 n) (as_seq h0 a) (v bBits) (as_seq h0 b))
-
-
-inline_for_extraction noextract
-val bn_check_mod_exp: #t:limb_t -> k:BM.mont t -> bn_check_mod_exp_st t k.BM.bn.BN.len
-
-
-// This function is *NOT* constant-time on the exponent b.
-inline_for_extraction noextract
-let bn_mod_exp_precompr2_st (t:limb_t) (len:BN.meta_len t) =
-    n:lbignum t len
-  -> a:lbignum t len
-  -> bBits:size_t{v bBits > 0}
-  -> b:lbignum t (blocks bBits (size (bits t)))
-  -> r2:lbignum t len
-  -> res:lbignum t len ->
-  Stack unit
-  (requires fun h ->
-    live h n /\ live h a /\ live h b /\ live h res /\ live h r2 /\
-    disjoint res a /\ disjoint res b /\ disjoint res n /\ disjoint n a /\
-    disjoint res r2 /\ disjoint a r2 /\ disjoint n r2)
-  (ensures  fun h0 _ h1 -> modifies (loc res) h0 h1 /\
-    as_seq h1 res ==
-    S.bn_mod_exp_precompr2 (v len) (as_seq h0 n) (as_seq h0 a) (v bBits) (as_seq h0 b) (as_seq h0 r2))
-
-
-inline_for_extraction noextract
-val bn_mod_exp_precompr2: #t:limb_t -> k:BM.mont t -> bn_mod_exp_precompr2_st t k.BM.bn.BN.len
-
-
-// This function is constant-time on the exponent b.
-inline_for_extraction noextract
-let bn_mod_exp_mont_ladder_precompr2_st (t:limb_t) (len:BN.meta_len t) =
-    n:lbignum t len
-  -> a:lbignum t len
-  -> bBits:size_t{v bBits > 0}
-  -> b:lbignum t (blocks bBits (size (bits t)))
-  -> r2:lbignum t len
-  -> res:lbignum t len ->
-  Stack unit
-  (requires fun h ->
-    live h n /\ live h a /\ live h b /\ live h res /\ live h r2 /\
-    disjoint res a /\ disjoint res b /\ disjoint res n /\ disjoint n a /\
-    disjoint res r2 /\ disjoint a r2 /\ disjoint n r2)
-  (ensures  fun h0 _ h1 -> modifies (loc res) h0 h1 /\
-    as_seq h1 res ==
-    S.bn_mod_exp_mont_ladder_precompr2 (v len) (as_seq h0 n) (as_seq h0 a) (v bBits) (as_seq h0 b) (as_seq h0 r2))
-
-
-inline_for_extraction noextract
-val bn_mod_exp_mont_ladder_precompr2: #t:limb_t -> k:BM.mont t -> bn_mod_exp_mont_ladder_precompr2_st t k.BM.bn.BN.len
-
 
 inline_for_extraction noextract
 let bn_mod_exp_st (t:limb_t) (len:BN.meta_len t) =
@@ -127,3 +66,56 @@ val bn_mod_exp_mont_ladder:
   -> k:BM.mont t
   -> bn_mod_exp_mont_ladder_precompr2:bn_mod_exp_mont_ladder_precompr2_st t k.BM.bn.BN.len ->
   bn_mod_exp_mont_ladder_st t k.BM.bn.BN.len
+
+
+inline_for_extraction noextract
+let bn_mod_exp_fw_st (t:limb_t) (len:BN.meta_len t) =
+    nBits:size_t{v nBits / bits t < v len}
+  -> n:lbignum t len
+  -> a:lbignum t len
+  -> bBits:size_t{0 < v bBits /\ bits t * v (blocks bBits (size (bits t))) <= max_size_t}
+  -> b:lbignum t (blocks bBits (size (bits t)))
+  -> l:size_t{0 < v l /\ v l < bits U32 /\ pow2 (v l) * v len <= max_size_t}
+  -> res:lbignum t len ->
+  Stack unit
+  (requires fun h ->
+    live h n /\ live h a /\ live h b /\ live h res /\
+    disjoint res a /\ disjoint res b /\ disjoint res n /\ disjoint n a)
+  (ensures  fun h0 _ h1 -> modifies (loc res) h0 h1 /\
+    as_seq h1 res == S.bn_mod_exp_fw (v len) (v nBits) (as_seq h0 n) (as_seq h0 a) (v bBits) (as_seq h0 b) (v l))
+
+
+// This function is *NOT* constant-time on the exponent b.
+inline_for_extraction noextract
+val bn_mod_exp_fw:
+    #t:limb_t
+  -> k:BM.mont t
+  -> bn_mod_exp_fw_precompr2:bn_mod_exp_fw_precompr2_st t k.BM.bn.BN.len ->
+  bn_mod_exp_fw_st t k.BM.bn.BN.len
+
+
+// This function is constant-time on the exponent b.
+inline_for_extraction noextract
+val bn_mod_exp_fw_ct:
+    #t:limb_t
+  -> k:BM.mont t
+  -> bn_mod_exp_fw_precompr2_ct:bn_mod_exp_fw_precompr2_st t k.BM.bn.BN.len ->
+  bn_mod_exp_fw_st t k.BM.bn.BN.len
+
+
+inline_for_extraction noextract
+class exp (t:limb_t) = {
+  mont: BM.mont t;
+  exp_check: bn_check_mod_exp_st t mont.BM.bn.BN.len;
+  mod_exp_precomp: bn_mod_exp_precompr2_st t mont.BM.bn.BN.len;
+  ct_mod_exp_precomp: bn_mod_exp_mont_ladder_precompr2_st t mont.BM.bn.BN.len;
+  mod_exp_fw_precomp: bn_mod_exp_fw_precompr2_st t mont.BM.bn.BN.len;
+  ct_mod_exp_fw_precomp: bn_mod_exp_fw_precompr2_st t mont.BM.bn.BN.len;
+}
+
+// A completely run-time-only instance where the functions above exist in the C code.
+inline_for_extraction noextract
+val mk_runtime_exp: #t:limb_t -> len:BN.meta_len t -> exp t
+
+val mk_runtime_exp_len_lemma: #t:limb_t -> len:BN.meta_len t ->
+  Lemma ((mk_runtime_exp #t len).mont.BM.bn.BN.len == len) [SMTPat (mk_runtime_exp #t len)]
