code/bignum/Hacl.Bignum4096.fst
@@ -5,7 +5,6 @@ open FStar.Mul
 module BN = Hacl.Bignum
 module BM = Hacl.Bignum.Montgomery
 module BE = Hacl.Bignum.Exponentiation
-module BP = Hacl.Bignum.ExponentiationPrecomp
 module BR = Hacl.Bignum.ModReduction
 module BI = Hacl.Bignum.ModInv
 
@@ -106,41 +105,21 @@ let mod_exp_mont_ladder_precompr2: BE.bn_mod_exp_mont_ladder_precompr2_st t_limb
   BE.bn_mod_exp_mont_ladder_precompr2 mont_inst
 
 [@CInline]
-let mod_exp_: BE.bn_mod_exp_st t_limbs n_limbs =
-  BE.bn_mod_exp mont_inst mod_exp_precompr2
+let mod_exp_fw_precompr2: BE.bn_mod_exp_fw_precompr2_st t_limbs n_limbs =
+  BE.bn_mod_exp_fw_precompr2 mont_inst
 
 [@CInline]
-let mod_exp_mont_ladder_: BE.bn_mod_exp_mont_ladder_st t_limbs n_limbs =
-  BE.bn_mod_exp_mont_ladder mont_inst mod_exp_mont_ladder_precompr2
-
-[@CInline]
-let mod_exp_fw_precompr2: BP.bn_mod_exp_fw_precompr2_st t_limbs n_limbs =
-  BP.bn_mod_exp_fw_precompr2 mont_inst
-
-[@CInline]
-let mod_exp_fw_precompr2_ct: BP.bn_mod_exp_fw_precompr2_st t_limbs n_limbs =
-  BP.bn_mod_exp_fw_precompr2_ct mont_inst
-
-[@CInline]
-let mod_exp_fw: BP.bn_mod_exp_fw_st t_limbs n_limbs =
-  BP.bn_mod_exp_fw mont_inst mod_exp_fw_precompr2
-
-[@CInline]
-let mod_exp_fw_ct: BP.bn_mod_exp_fw_st t_limbs n_limbs =
-  BP.bn_mod_exp_fw_ct mont_inst mod_exp_fw_precompr2_ct
+let mod_exp_fw_precompr2_ct: BE.bn_mod_exp_fw_precompr2_st t_limbs n_limbs =
+  BE.bn_mod_exp_fw_precompr2_ct mont_inst
 
 inline_for_extraction noextract
-instance exp_inst: BP.exp t_limbs = {
-  BP.mont = mont_inst;
-  BP.exp_check;
-  BP.mod_exp_precomp = mod_exp_precompr2;
-  BP.ct_mod_exp_precomp = mod_exp_mont_ladder_precompr2;
-  BP.mod_exp = mod_exp_;
-  BP.ct_mod_exp = mod_exp_mont_ladder_;
-  BP.mod_exp_fw_precomp = mod_exp_fw_precompr2;
-  BP.ct_mod_exp_fw_precomp = mod_exp_fw_precompr2_ct;
-  BP.mod_exp_fw = mod_exp_fw;
-  BP.ct_mod_exp_fw = mod_exp_fw_ct;
+instance exp_inst: BE.exp t_limbs = {
+  BE.mont = mont_inst;
+  BE.exp_check;
+  BE.mod_exp_precomp = mod_exp_precompr2;
+  BE.ct_mod_exp_precomp = mod_exp_mont_ladder_precompr2;
+  BE.mod_exp_fw_precomp = mod_exp_fw_precompr2;
+  BE.ct_mod_exp_fw_precomp = mod_exp_fw_precompr2_ct;
 }
 
 let mod_exp = BS.bn_mod_exp_safe exp_inst
