code/bignum/Hacl.Spec.Bignum.Exponentiation.fsti
@@ -6,102 +6,12 @@ open Lib.IntTypes
 open Lib.Sequence
 
 open Hacl.Spec.Bignum.Definitions
+include Hacl.Spec.Bignum.ExpBM
+include Hacl.Spec.Bignum.ExpFW
 
 module BM = Hacl.Spec.Bignum.Montgomery
 
 #reset-options "--z3rlimit 50 --fuel 0 --ifuel 0"
-
-
-let bn_mod_exp_pre
-  (#t:limb_t)
-  (#nLen:size_pos{2 * bits t * nLen <= max_size_t})
-  (n:lbignum t nLen)
-  (a:lbignum t nLen)
-  (bBits:size_pos)
-  (b:lbignum t (blocks bBits (bits t)))
- =
-   bn_v n % 2 = 1 /\ 1 < bn_v n /\
-   0 < bn_v b /\ bn_v b < pow2 bBits /\ bn_v a < bn_v n
-
-
-let bn_mod_exp_post
-  (#t:limb_t)
-  (#nLen:size_pos{2 * bits t * nLen <= max_size_t})
-  (n:lbignum t nLen)
-  (a:lbignum t nLen)
-  (bBits:size_pos)
-  (b:lbignum t (blocks bBits (bits t)))
-  (res:lbignum t nLen)
- =
-  bn_mod_exp_pre n a bBits b /\
-  bn_v res == Lib.NatMod.pow_mod #(bn_v n) (bn_v a) (bn_v b)
-
-
-val bn_check_mod_exp:
-    #t:limb_t
-  -> #nLen:size_pos{2 * bits t * nLen <= max_size_t}
-  -> n:lbignum t nLen
-  -> a:lbignum t nLen
-  -> bBits:size_pos
-  -> b:lbignum t (blocks bBits (bits t)) ->
-  res:limb t{
-    let b = bn_v n % 2 = 1 && 1 < bn_v n && 0 < bn_v b && bn_v b < pow2 bBits && bn_v a < bn_v n in
-    v res == (if b then v (ones t SEC) else v (zeros t SEC))}
-
-
-// This function is *NOT* constant-time on the exponent b
-val bn_mod_exp_precompr2:
-    #t:limb_t
-  -> nLen:size_pos{2 * bits t * nLen <= max_size_t}
-  -> n:lbignum t nLen
-  -> a:lbignum t nLen
-  -> bBits:size_pos
-  -> b:lbignum t (blocks bBits (bits t))
-  -> r2:lbignum t nLen ->
-  lbignum t nLen
-
-
-val bn_mod_exp_precompr2_lemma:
-    #t:limb_t
-  -> nLen:size_pos{2 * bits t * nLen <= max_size_t}
-  -> n:lbignum t nLen
-  -> a:lbignum t nLen
-  -> bBits:size_pos
-  -> b:lbignum t (blocks bBits (bits t))
-  -> r2:lbignum t nLen -> Lemma
-  (requires
-    bn_mod_exp_pre n a bBits b /\
-    bn_v r2 == pow2 (2 * bits t * nLen) % bn_v n)
-  (ensures
-    bn_mod_exp_post n a bBits b (bn_mod_exp_precompr2 nLen n a bBits b r2))
-
-
-// This function is constant-time on the exponent b
-val bn_mod_exp_mont_ladder_precompr2:
-    #t:limb_t
-  -> nLen:size_pos{2 * bits t * nLen <= max_size_t}
-  -> n:lbignum t nLen
-  -> a:lbignum t nLen
-  -> bBits:size_pos
-  -> b:lbignum t (blocks bBits (bits t))
-  -> r2:lbignum t nLen ->
-  lbignum t nLen
-
-
-val bn_mod_exp_mont_ladder_precompr2_lemma:
-    #t:limb_t
-  -> nLen:size_pos{2 * bits t * nLen <= max_size_t}
-  -> n:lbignum t nLen
-  -> a:lbignum t nLen
-  -> bBits:size_pos
-  -> b:lbignum t (blocks bBits (bits t))
-  -> r2:lbignum t nLen -> Lemma
-  (requires
-    bn_mod_exp_pre n a bBits b /\
-    bn_v r2 == pow2 (2 * bits t * nLen) % bn_v n)
-  (ensures
-    bn_mod_exp_post n a bBits b (bn_mod_exp_mont_ladder_precompr2 nLen n a bBits b r2))
-
 
 // This function is *NOT* constant-time on the exponent b
 val bn_mod_exp:
@@ -149,3 +59,28 @@ val bn_mod_exp_mont_ladder_lemma:
   -> b:lbignum t (blocks bBits (bits t)) -> Lemma
   (requires bn_mod_exp_pre n a bBits b /\ pow2 nBits < bn_v n)
   (ensures  bn_mod_exp_post n a bBits b (bn_mod_exp_mont_ladder nLen nBits n a bBits b))
+
+
+val bn_mod_exp_fw:
+    #t:limb_t
+  -> nLen:size_pos{2 * bits t * nLen <= max_size_t}
+  -> nBits:size_nat{nBits / bits t < nLen}
+  -> n:lbignum t nLen
+  -> a:lbignum t nLen
+  -> bBits:size_pos
+  -> b:lbignum t (blocks bBits (bits t))
+  -> l:size_pos{l <= bits t /\ pow2 l * nLen <= max_size_t} ->
+  lbignum t nLen
+
+
+val bn_mod_exp_fw_lemma:
+    #t:limb_t
+  -> nLen:size_pos{2 * bits t * nLen <= max_size_t}
+  -> nBits:size_nat{nBits / bits t < nLen}
+  -> n:lbignum t nLen
+  -> a:lbignum t nLen
+  -> bBits:size_pos
+  -> b:lbignum t (blocks bBits (bits t))
+  -> l:size_pos{l <= bits t /\ pow2 l * nLen <= max_size_t} -> Lemma
+  (requires bn_mod_exp_pre n a bBits b /\ pow2 nBits < bn_v n)
+  (ensures  bn_mod_exp_post n a bBits b (bn_mod_exp_fw nLen nBits n a bBits b l))
