code/bignum/Hacl.Bignum.ExpBM.fsti
@@ -1,0 +1,79 @@
+module Hacl.Bignum.ExpBM
+
+open FStar.HyperStack
+open FStar.HyperStack.ST
+open FStar.Mul
+
+open Lib.IntTypes
+open Lib.Buffer
+
+open Hacl.Bignum.Definitions
+
+module S = Hacl.Spec.Bignum.ExpBM
+module BN = Hacl.Bignum
+module BM = Hacl.Bignum.Montgomery
+
+#reset-options "--z3rlimit 50 --fuel 0 --ifuel 0"
+
+
+inline_for_extraction noextract
+let bn_check_mod_exp_st (t:limb_t) (len:BN.meta_len t) =
+    n:lbignum t len
+  -> a:lbignum t len
+  -> bBits:size_t{0 < v bBits /\ bits t * v (blocks bBits (size (bits t))) <= max_size_t}
+  -> b:lbignum t (blocks bBits (size (bits t))) ->
+  Stack (limb t)
+  (requires fun h ->
+    live h n /\ live h a /\ live h b)
+  (ensures  fun h0 r h1 -> modifies0 h0 h1 /\
+    r == S.bn_check_mod_exp (as_seq h0 n) (as_seq h0 a) (v bBits) (as_seq h0 b))
+
+
+inline_for_extraction noextract
+val bn_check_mod_exp: #t:limb_t -> k:BM.mont t -> bn_check_mod_exp_st t k.BM.bn.BN.len
+
+
+// This function is *NOT* constant-time on the exponent b.
+inline_for_extraction noextract
+let bn_mod_exp_precompr2_st (t:limb_t) (len:BN.meta_len t) =
+    n:lbignum t len
+  -> a:lbignum t len
+  -> bBits:size_t{v bBits > 0}
+  -> b:lbignum t (blocks bBits (size (bits t)))
+  -> r2:lbignum t len
+  -> res:lbignum t len ->
+  Stack unit
+  (requires fun h ->
+    live h n /\ live h a /\ live h b /\ live h res /\ live h r2 /\
+    disjoint res a /\ disjoint res b /\ disjoint res n /\ disjoint n a /\
+    disjoint res r2 /\ disjoint a r2 /\ disjoint n r2)
+  (ensures  fun h0 _ h1 -> modifies (loc res) h0 h1 /\
+    as_seq h1 res ==
+    S.bn_mod_exp_precompr2 (v len) (as_seq h0 n) (as_seq h0 a) (v bBits) (as_seq h0 b) (as_seq h0 r2))
+
+
+inline_for_extraction noextract
+val bn_mod_exp_precompr2: #t:limb_t -> k:BM.mont t -> bn_mod_exp_precompr2_st t k.BM.bn.BN.len
+
+
+// This function is constant-time on the exponent b.
+inline_for_extraction noextract
+let bn_mod_exp_mont_ladder_precompr2_st (t:limb_t) (len:BN.meta_len t) =
+    n:lbignum t len
+  -> a:lbignum t len
+  -> bBits:size_t{v bBits > 0}
+  -> b:lbignum t (blocks bBits (size (bits t)))
+  -> r2:lbignum t len
+  -> res:lbignum t len ->
+  Stack unit
+  (requires fun h ->
+    live h n /\ live h a /\ live h b /\ live h res /\ live h r2 /\
+    disjoint res a /\ disjoint res b /\ disjoint res n /\ disjoint n a /\
+    disjoint res r2 /\ disjoint a r2 /\ disjoint n r2)
+  (ensures  fun h0 _ h1 -> modifies (loc res) h0 h1 /\
+    as_seq h1 res ==
+    S.bn_mod_exp_mont_ladder_precompr2 (v len) (as_seq h0 n) (as_seq h0 a) (v bBits) (as_seq h0 b) (as_seq h0 r2))
+
+
+inline_for_extraction noextract
+val bn_mod_exp_mont_ladder_precompr2: #t:limb_t -> k:BM.mont t -> bn_mod_exp_mont_ladder_precompr2_st t k.BM.bn.BN.len
