code/bignum/Hacl.Bignum.Montgomery.fst
@@ -145,13 +145,14 @@ let bn_mont_sqr #t k mont_reduction n nInv_u64 aM resM =
   mont_reduction n nInv_u64 c resM;
   pop_frame ()
 
+
 /// All of the functions above are inline_for_extraction noextract meaning that
 /// they're intended to be specialized by clients for a specific value of
 /// ``len``. We provide a default implementation that actually keeps ``len`` at
 /// runtime, to offer a version of mod_exp where all the parameters are present
 /// at run-time.
 [@CInline]
-let bn_check_modulus_u32 (len: BN.meta_len U32) : bn_check_modulus_st U32 len =
+let bn_check_modulus_u32 (len:BN.meta_len U32) : bn_check_modulus_st U32 len =
   bn_check_modulus #U32 #len
 [@CInline]
 let bn_precomp_r2_mod_n_u32 (len:BN.meta_len U32) : bn_precomp_r2_mod_n_st U32 len =
@@ -160,20 +161,20 @@ let bn_precomp_r2_mod_n_u32 (len:BN.meta_len U32) : bn_precomp_r2_mod_n_st U32 l
 let bn_mont_reduction_u32 (len:BN.meta_len U32) : bn_mont_reduction_st U32 len =
   bn_mont_reduction (BN.mk_runtime_bn U32 len)
 [@CInline]
-let bn_to_mont_u32 (len: BN.meta_len U32) : bn_to_mont_st U32 len =
+let bn_to_mont_u32 (len:BN.meta_len U32) : bn_to_mont_st U32 len =
   bn_to_mont (BN.mk_runtime_bn U32 len) (bn_mont_reduction_u32 len)
 [@CInline]
-let bn_from_mont_u32 (len: BN.meta_len U32) : bn_from_mont_st U32 len =
+let bn_from_mont_u32 (len:BN.meta_len U32) : bn_from_mont_st U32 len =
   bn_from_mont (BN.mk_runtime_bn U32 len) (bn_mont_reduction_u32 len)
 [@CInline]
-let bn_mont_mul_u32 (len: BN.meta_len U32) : bn_mont_mul_st U32 len =
+let bn_mont_mul_u32 (len:BN.meta_len U32) : bn_mont_mul_st U32 len =
   bn_mont_mul (BN.mk_runtime_bn U32 len) (bn_mont_reduction_u32 len)
 [@CInline]
-let bn_mont_sqr_32 (len: BN.meta_len U32) : bn_mont_sqr_st U32 len =
+let bn_mont_sqr_u32 (len:BN.meta_len U32) : bn_mont_sqr_st U32 len =
   bn_mont_sqr (BN.mk_runtime_bn U32 len) (bn_mont_reduction_u32 len)
 
 inline_for_extraction noextract
-let mk_runtime_mont_u32 (len: BN.meta_len U32) : mont U32 = {
+let mk_runtime_mont_u32 (len:BN.meta_len U32) : mont U32 = {
   bn = BN.mk_runtime_bn U32 len;
   mont_check = bn_check_modulus_u32 len;
   precomp = bn_precomp_r2_mod_n_u32 len;
@@ -181,11 +182,12 @@ let mk_runtime_mont_u32 (len: BN.meta_len U32) : mont U32 = {
   to = bn_to_mont_u32 len;
   from = bn_from_mont_u32 len;
   mul = bn_mont_mul_u32 len;
-  sqr = bn_mont_sqr_32 len;
+  sqr = bn_mont_sqr_u32 len;
 }
 
+
 [@CInline]
-let bn_check_modulus_u64 (len: BN.meta_len U64) : bn_check_modulus_st U64 len =
+let bn_check_modulus_u64 (len:BN.meta_len U64) : bn_check_modulus_st U64 len =
   bn_check_modulus #U64 #len
 [@CInline]
 let bn_precomp_r2_mod_n_u64 (len:BN.meta_len U64) : bn_precomp_r2_mod_n_st U64 len =
@@ -194,20 +196,20 @@ let bn_precomp_r2_mod_n_u64 (len:BN.meta_len U64) : bn_precomp_r2_mod_n_st U64 l
 let bn_mont_reduction_u64 (len:BN.meta_len U64) : bn_mont_reduction_st U64 len =
   bn_mont_reduction (BN.mk_runtime_bn U64 len)
 [@CInline]
-let bn_to_mont_u64 (len: BN.meta_len U64) : bn_to_mont_st U64 len =
+let bn_to_mont_u64 (len:BN.meta_len U64) : bn_to_mont_st U64 len =
   bn_to_mont (BN.mk_runtime_bn U64 len) (bn_mont_reduction_u64 len)
 [@CInline]
-let bn_from_mont_u64 (len: BN.meta_len U64) : bn_from_mont_st U64 len =
+let bn_from_mont_u64 (len:BN.meta_len U64) : bn_from_mont_st U64 len =
   bn_from_mont (BN.mk_runtime_bn U64 len) (bn_mont_reduction_u64 len)
 [@CInline]
-let bn_mont_mul_u64 (len: BN.meta_len U64) : bn_mont_mul_st U64 len =
+let bn_mont_mul_u64 (len:BN.meta_len U64) : bn_mont_mul_st U64 len =
   bn_mont_mul (BN.mk_runtime_bn U64 len) (bn_mont_reduction_u64 len)
 [@CInline]
-let bn_mont_sqr_64 (len: BN.meta_len U64) : bn_mont_sqr_st U64 len =
+let bn_mont_sqr_u64 (len:BN.meta_len U64) : bn_mont_sqr_st U64 len =
   bn_mont_sqr (BN.mk_runtime_bn U64 len) (bn_mont_reduction_u64 len)
 
 inline_for_extraction noextract
-let mk_runtime_mont_u64 (len: BN.meta_len U64) : mont U64 = {
+let mk_runtime_mont_u64 (len:BN.meta_len U64) : mont U64 = {
   bn = BN.mk_runtime_bn U64 len;
   mont_check = bn_check_modulus_u64 len;
   precomp = bn_precomp_r2_mod_n_u64 len;
@@ -215,9 +217,8 @@ let mk_runtime_mont_u64 (len: BN.meta_len U64) : mont U64 = {
   to = bn_to_mont_u64 len;
   from = bn_from_mont_u64 len;
   mul = bn_mont_mul_u64 len;
-  sqr = bn_mont_sqr_64 len;
+  sqr = bn_mont_sqr_u64 len;
 }
-
 
 let mk_runtime_mont (#t:limb_t) (len:BN.meta_len t) : mont t =
   match t with
